src/SelfClose.v
@@ -1,0 +1,153 @@
+Require Import Common.
+Require Import Psatz.
+
+Require Import Utopia.
+Require Import Monads.
+
+Definition function_name := nat.
+
+Inductive expr :=
+| Arg : expr
+| Self : expr
+| Deref : expr -> nat -> expr
+| Call : expr -> expr -> expr
+| Constr (tag : nat) (args : list expr)
+| Switch (cases : list expr)
+| Close (f : function_name) (free : list expr)
+.
+
+Definition env := list expr.
+
+Inductive value : expr -> Prop :=
+| VConstr : forall tag args, Forall value args -> value (Constr tag args)
+| VClose : forall f free, Forall value free -> value (Close f free).
+
+(* Continuation-based step relation *)
+
+Inductive state :=
+| Run (e : expr) (a : expr) (s : expr) (k : expr -> state)
+| Stop (e : expr).
+
+Inductive sstep (E : env) : state -> state -> Prop :=
+| SArg : forall a s k,
+        sstep E (Run Arg a s k) (k a)
+| SSelf : forall a s k,
+        sstep E (Run Self a s k) (k s)
+
+| SDerefStep : forall e off a s k,
+        ~ value e ->
+        sstep E (Run (Deref e off) a s k)
+                (Run e a s (fun v => Run (Deref v off) a s k))
+| SDerefinateConstr : forall tag args off a s k v,
+        Forall value args ->
+        nth_error args off = Some v ->
+        sstep E (Run (Deref (Constr tag args) off) a s k) (k v)
+| SDerefinateClose : forall fname free off a s k v,
+        Forall value free ->
+        nth_error free off = Some v ->
+        sstep E (Run (Deref (Close fname free) off) a s k) (k v)
+
+| SConstrStep : forall fname vs e es a s k,
+        Forall value vs ->
+        ~ value e ->
+        sstep E (Run (Constr fname (vs ++ [e] ++ es)) a s k)
+                (Run e a s (fun v => Run (Constr fname (vs ++ [v] ++ es)) a s k))
+| SConstrDone : forall fname vs a s k,
+        Forall value vs ->
+        sstep E (Run (Constr fname vs) a s k) (k (Constr fname vs))
+
+| SCloseStep : forall fname vs e es a s k,
+        Forall value vs ->
+        ~ value e ->
+        sstep E (Run (Close fname (vs ++ [e] ++ es)) a s k)
+                (Run e a s (fun v => Run (Close fname (vs ++ [v] ++ es)) a s k))
+| SCloseDone : forall fname vs a s k,
+        Forall value vs ->
+        sstep E (Run (Close fname vs) a s k) (k (Close fname vs))
+
+| SCallL : forall e1 e2 a s k,
+        ~ value e1 ->
+        sstep E (Run (Call e1 e2) a s k)
+                (Run e1 a s (fun v => Run (Call v e2) a s k))
+| SCallR : forall e1 e2 a s k,
+        value e1 ->
+        ~ value e2 ->
+        sstep E (Run (Call e1 e2) a s k)
+                (Run e2 a s (fun v => Run (Call e1 v) a s k))
+| SMakeCall : forall fname free arg a s k body,
+        Forall value free ->
+        value arg ->
+        nth_error E fname = Some body ->
+        sstep E (Run (Call (Close fname free) arg) a s k)
+                (Run body arg (Close fname free) k)
+
+| SSwitchinate : forall cases tag args s k case,
+        nth_error cases tag = Some case ->
+        sstep E (Run (Switch cases) (Constr tag args) s k)
+                (Run case (Constr tag args) s k)
+.
+
+Inductive sstar (E : env) : state -> state -> Prop :=
+| SStarNil : forall e, sstar E e e
+| SStarCons : forall e e' e'',
+        sstep E e e' ->
+        sstar E e' e'' ->
+        sstar E e e''.
+
+Inductive splus (E : env) : state -> state -> Prop :=
+| SPlusOne : forall s s',
+        sstep E s s' ->
+        splus E s s'
+| SPlusCons : forall s s' s'',
+        sstep E s s' ->
+        splus E s' s'' ->
+        splus E s s''.
+
+
+
+(*
+ * Mutual recursion/induction schemes for expr
+ *)
+
+Definition expr_rect_mut
+        (P : expr -> Type)
+        (Pl : list expr -> Type)
+    (HArg :     P Arg)
+    (HSelf :    P Self)
+    (HDeref :   forall e off, P e -> P (Deref e off))
+    (HCall :    forall f a, P f -> P a -> P (Call f a))
+    (HConstr :  forall tag args, Pl args -> P (Constr tag args))
+    (HSwitch :  forall cases, Pl cases -> P (Switch cases))
+    (HClose :   forall f free, Pl free -> P (Close f free))
+    (Hnil :     Pl [])
+    (Hcons :    forall e es, P e -> Pl es -> Pl (e :: es))
+    (e : expr) : P e :=
+    let fix go e :=
+        let fix go_list es :=
+            match es as es_ return Pl es_ with
+            | [] => Hnil
+            | e :: es => Hcons e es (go e) (go_list es)
+            end in
+        match e as e_ return P e_ with
+        | Arg => HArg
+        | Self => HSelf
+        | Deref e off => HDeref e off (go e)
+        | Call f a => HCall f a (go f) (go a)
+        | Constr tag args => HConstr tag args (go_list args)
+        | Switch cases => HSwitch cases (go_list cases)
+        | Close f free => HClose f free (go_list free)
+        end in go e.
+
+(* Useful wrapper for `expr_rect_mut with (Pl := Forall P)` *)
+Definition expr_ind' (P : expr -> Prop)
+    (HArg :     P Arg)
+    (HSelf :    P Self)
+    (HDeref :   forall e off, P e -> P (Deref e off))
+    (HCall :    forall f a, P f -> P a -> P (Call f a))
+    (HConstr :  forall tag args, Forall P args -> P (Constr tag args))
+    (HSwitch :  forall cases, Forall P cases -> P (Switch cases))
+    (HClose :   forall f free, Forall P free -> P (Close f free))
+    (e : expr) : P e :=
+    ltac:(refine (@expr_rect_mut P (Forall P)
+        HArg HSelf HDeref HCall HConstr HSwitch HClose _ _ e); eauto).
+
