src/SelfCloseComp.v
@@ -1,0 +1,264 @@
+Require Import Common Monads.
+Require Import Metadata.
+Require String.
+Require Switched SelfClose.
+Require Import ListLemmas.
+
+Require Import Psatz.
+
+Module A := Switched.
+Module B := SelfClose.
+
+
+Definition compile :=
+    let fix go e :=
+        let fix go_list es :=
+            match es with
+            | [] => []
+            | e :: es => go e :: go_list es
+            end in
+        match e with
+        | A.Arg => B.Arg
+        | A.UpVar n => B.Deref B.Self n
+        | A.Deref e off => B.Deref (go e) off
+        | A.Call f a => B.Call (go f) (go a)
+        | A.Constr tag args => B.Constr tag (go_list args)
+        | A.Switch cases => B.Switch (go_list cases)
+        | A.Close fname free => B.Close fname (go_list free)
+        end in go.
+
+Definition compile_list :=
+    let go := compile in
+    let fix go_list es :=
+        match es with
+        | [] => []
+        | e :: es => go e :: go_list es
+        end in go_list.
+
+Ltac refold_compile :=
+    fold compile_list in *.
+
+
+Definition compile_cu (cu : list A.expr * list metadata) : list B.expr * list metadata :=
+    let '(exprs, metas) := cu in
+    let exprs' := compile_list exprs in
+    (exprs', metas).
+
+
+Lemma compile_list_Forall : forall aes bes,
+    compile_list aes = bes ->
+    Forall2 (fun a b => compile a = b) aes bes.
+induction aes; destruct bes; intros0 Hcomp; simpl in Hcomp; try discriminate.
+- constructor.
+- invc Hcomp. eauto.
+Qed.
+
+Lemma compile_list_length : forall es,
+    length (compile_list es) = length es.
+intros. induction es.
+- reflexivity.
+- simpl. f_equal. eauto.
+Qed.
+
+
+
+
+
+
+Inductive I_expr : A.expr -> B.expr -> Prop :=
+| IArg : I_expr A.Arg B.Arg
+| IUpVar : forall n,
+        I_expr (A.UpVar n)
+               (B.Deref B.Self n)
+| IDeref : forall ae be off,
+        I_expr ae be ->
+        I_expr (A.Deref ae off)
+               (B.Deref be off)
+| ICall : forall af aa bf ba,
+        I_expr af bf ->
+        I_expr aa ba ->
+        I_expr (A.Call af aa) (B.Call bf ba)
+| IConstr : forall tag aargs bargs,
+        Forall2 I_expr aargs bargs ->
+        I_expr (A.Constr tag aargs) (B.Constr tag bargs)
+| IElimBody : forall acases bcases,
+        Forall2 I_expr acases bcases ->
+        I_expr (A.Switch acases) (B.Switch bcases)
+| IClose : forall fname afree bfree,
+        Forall2 (I_expr) afree bfree ->
+        I_expr (A.Close fname afree) (B.Close fname bfree)
+.
+
+Inductive I : A.state -> B.state -> Prop :=
+| IRun : forall ae al ak be ba fname free bk,
+        I_expr ae be ->
+        Forall2 I_expr al (ba :: free) ->
+        Forall A.value al ->
+        B.value ba ->
+        Forall B.value free ->
+        (forall av bv,
+            A.value av ->
+            B.value bv ->
+            I_expr av bv ->
+            I (ak av) (bk bv)) ->
+        I (A.Run ae al ak) (B.Run be ba (B.Close fname free) bk)
+
+| IStop : forall ae be,
+        I_expr ae be ->
+        I (A.Stop ae) (B.Stop be).
+
+
+
+Lemma I_expr_value : forall a b,
+    I_expr a b ->
+    A.value a ->
+    B.value b.
+induction a using A.expr_ind'; intros0 II Aval; invc Aval; invc II.
+- constructor. list_magic_on (args, (bargs, tt)).
+- constructor. list_magic_on (free, (bfree, tt)).
+Qed.
+Hint Resolve I_expr_value.
+
+Lemma I_expr_value' : forall b a,
+    I_expr a b ->
+    B.value b ->
+    A.value a.
+induction b using B.expr_ind'; intros0 II Bval; invc Bval; invc II.
+- constructor. list_magic_on (args, (aargs, tt)).
+- constructor. list_magic_on (free, (afree, tt)).
+Qed.
+
+Lemma I_expr_not_value : forall a b,
+    I_expr a b ->
+    ~A.value a ->
+    ~B.value b.
+intros. intro. fwd eapply I_expr_value'; eauto.
+Qed.
+Hint Resolve I_expr_not_value.
+
+Lemma I_expr_not_value' : forall a b,
+    I_expr a b ->
+    ~B.value b ->
+    ~A.value a.
+intros. intro. fwd eapply I_expr_value; eauto.
+Qed.
+
+Lemma Forall_I_expr_value : forall aes bes,
+    Forall2 I_expr aes bes ->
+    Forall A.value aes ->
+    Forall B.value bes.
+intros. list_magic_on (aes, (bes, tt)).
+Qed.
+Hint Resolve Forall_I_expr_value.
+
+
+
+Theorem compile_I_expr : forall ae be,
+    compile ae = be ->
+    I_expr ae be.
+induction ae using A.expr_rect_mut with
+    (Pl := fun aes => forall bes,
+        compile_list aes = bes ->
+        Forall2 I_expr aes bes);
+intros0 Hcomp;
+simpl in Hcomp; refold_compile; try rewrite <- Hcomp in *;
+try solve [eauto | constructor; eauto].
+Qed.
+
+
+
+Ltac i_ctor := intros; constructor; eauto.
+Ltac i_lem H := intros; eapply H; eauto.
+
+Theorem I_sim : forall AE BE a a' b,
+    compile_list AE = BE ->
+    I a b ->
+    A.sstep AE a a' ->
+    exists b',
+        B.splus BE b b' /\
+        I a' b'.
+
+destruct a as [ae al ak | ae];
+intros0 Henv II Astep; [ | solve [invc Astep] ].
+
+inv Astep; invc II; try on (I_expr _ _), invc.
+
+- on (Forall2 _ _ (_ :: _)), invc. simpl in *. inject_some.
+  on (Forall _ (_ :: _)), invc.
+
+  eexists. split. eapply B.SPlusOne, B.SArg.
+  on _, eapply_; eauto.
+
+- on (Forall2 _ _ (_ :: _)), invc. simpl in *.
+  on (Forall _ (_ :: _)), invc.
+  fwd eapply Forall2_nth_error_ex as HH; eauto.
+    destruct HH as (bv & ? & ?).
+  assert (A.value v).  { eapply Forall_nth_error; eauto. }
+
+  eexists. split.
+    { eapply B.SPlusCons. eapply B.SDerefStep. inversion 1.
+      eapply B.SPlusCons. eapply B.SSelf.
+      eapply B.SPlusOne.  eapply B.SDerefinateClose; eauto. }
+  on _, eapply_; eauto.
+
+- eexists. split. eapply B.SPlusOne, B.SDerefStep; eauto.
+  i_ctor. i_ctor. i_ctor.
+
+- on (I_expr (A.Constr _ _) _), invc.
+  assert (A.value v).  { eapply Forall_nth_error with (xs := args); eauto. }
+  fwd eapply Forall2_nth_error_ex; eauto. break_exists. break_and.
+
+  eexists. split. eapply B.SPlusOne, B.SDerefinateConstr; eauto.
+  on _, eapply_; eauto.
+
+- on (I_expr (A.Close _ _) _), invc.
+  assert (A.value v).  { eapply Forall_nth_error with (xs := free); eauto. }
+  fwd eapply Forall2_nth_error_ex; eauto. break_exists. break_and.
+
+  eexists. split. eapply B.SPlusOne, B.SDerefinateClose; eauto.
+  on _, eapply_; eauto.
+
+- on _, invc_using Forall2_3part_inv.
+
+  eexists. split. eapply B.SPlusOne, B.SConstrStep; eauto.
+  i_ctor. i_ctor. i_ctor. eauto using Forall2_app.
+
+- eexists. split. eapply B.SPlusOne, B.SConstrDone; eauto.
+  on _, eapply_; eauto.
+  all: constructor; eauto.
+
+- on _, invc_using Forall2_3part_inv.
+
+  eexists. split. eapply B.SPlusOne, B.SCloseStep; eauto.
+  i_ctor. i_ctor. i_ctor. eauto using Forall2_app.
+
+- eexists. split. eapply B.SPlusOne, B.SCloseDone; eauto.
+  on _, eapply_; eauto.
+  all: constructor; eauto.
+
+- eexists. split. eapply B.SPlusOne, B.SCallL; eauto.
+  i_ctor. i_ctor. i_ctor.
+
+- eexists. split. eapply B.SPlusOne, B.SCallR; eauto.
+  i_ctor. i_ctor. i_ctor.
+
+- fwd eapply Forall2_nth_error_ex with (xs := AE) (ys := compile_list AE); eauto.
+    { eapply compile_list_Forall. reflexivity. }
+    break_exists. break_and.
+  on (I_expr (A.Close _ _) _), invc.
+
+  eexists. split. eapply B.SPlusOne, B.SMakeCall; eauto using compile_I_expr.
+  i_ctor. eauto using compile_I_expr.
+
+- fwd eapply Forall2_nth_error_ex with (xs := cases); eauto.
+    break_exists. break_and.
+  on (Forall2 _ (_ :: _) _), invc.
+  on (Forall _ (_ :: _)), invc.
+  on (A.value (A.Constr _ _)), invc.
+  on (I_expr (A.Constr _ _) _), invc.
+
+  eexists. split. eapply B.SPlusOne, B.SSwitchinate; eauto.
+  i_ctor.
+  + i_ctor. i_ctor.
+  + i_ctor. i_ctor.
+Qed.
